steel/Veritas.Steel.Verifier.fsti
@@ -1,0 +1,247 @@
+module Veritas.Steel.Verifier
+open Steel.Effect
+open Steel.Effect.Atomic
+open Steel.Memory
+open Steel.FractionalPermission
+open FStar.Ghost
+module U32 = FStar.UInt32
+module U64 = FStar.UInt64
+open Veritas.Steel.VCache
+open Veritas.Steel.Types
+open Steel.Reference
+let thread_id = U32.t
+let counter_t = ref U64.t
+val prf_set_hash : Type0
+val prf_set_hash_inv (_:prf_set_hash) : slprop u#1
+
+noeq
+type thread_state_t = {
+  id           : thread_id;
+  st           : vstore;  //a map from keys (cache ids) to merkle leaf or internal nodes
+  clock        : counter_t;
+  hadd         : prf_set_hash; //current incremental set hash values; TODO
+  hevict       : prf_set_hash;
+  failed       : ref bool
+}
+
+[@@erasable]
+noeq
+type thread_state_model = {
+  model_failed : bool;
+  model_store : VCache.contents;
+  model_clock : erased U64.t;
+//add sets to model hash state
+}
+
+[@@__reduce__]
+let thread_state_inv (t:thread_state_t) (m:thread_state_model)
+  : slprop
+  = VCache.is_vstore t.st m.model_store `star`
+    pts_to t.clock full_perm m.model_clock `star`
+    pts_to t.failed full_perm m.model_failed
+
+let change_slprop (#[@@framing_implicit] p:slprop)
+                  (#[@@framing_implicit] q:slprop)
+                  (_:unit)
+  : Steel unit p (fun _ -> q) (requires fun _ -> p==q) (ensures fun _ _ _ -> True)
+  = Steel.Effect.change_slprop p q (fun _ -> ())
+
+val sladmit (#[@@framing_implicit] p:slprop)
+            (#[@@framing_implicit] q:slprop)
+            (_:unit)
+  : SteelT unit p (fun _ -> q)
+
+let model_fail tsm = {tsm with model_failed=false}
+
+let fail (#tsm:_) (vs:thread_state_t) (msg:string)
+  : SteelT unit
+    (thread_state_inv vs tsm)
+    (fun _ -> thread_state_inv vs (model_fail tsm))
+  = let _ = Steel.Reference.write vs.failed false in ()
+
+let slot (tsm:thread_state_model) = VCache.slot_id tsm.model_store
+
+let vget_model tsm (s:slot tsm) (v:value) : thread_state_model =
+  match Seq.index tsm.model_store (U32.v s) with
+  | None -> model_fail tsm
+  | Some r' ->
+    if v = r'.record_value then tsm else model_fail tsm
+
+let vget (#tsm:_) (s:slot tsm) (v:value) (vs: thread_state_t)
+  : SteelT unit
+    (requires thread_state_inv vs tsm)
+    (ensures fun _ -> thread_state_inv vs (vget_model tsm s v))
+  = let ro = VCache.vcache_get_record vs.st s in
+    match ro with
+    | None ->
+      fail vs "Slot not found";
+      change_slprop ()
+    | Some r' ->
+      if v = r'.record_value
+      then (change_slprop #(thread_state_inv vs tsm) #(thread_state_inv vs (vget_model tsm s v)) (); ())
+      else (fail vs "Failed: inconsistent key or value in Get";
+            change_slprop())
+
+let model_get_record (tsm:thread_state_model) (s:slot tsm)
+  : GTot (option record)
+  = Seq.index tsm.model_store (U32.v s)
+
+let model_put_record (tsm:thread_state_model) (s:slot tsm) (r:record)
+  : thread_state_model
+  = {tsm with model_store=Seq.upd tsm.model_store (U32.v s) (Some r)}
+
+let vput_model (tsm:thread_state_model) (s:slot tsm) (v:value)
+  : thread_state_model
+  = match model_get_record tsm s with
+    | None -> model_fail tsm
+    | Some r -> model_put_record tsm s ({r with record_value=v})
+
+(* verifier write operation *)
+let vput (#tsm:_) (s:slot tsm) (v:value) (vs: thread_state_t)
+  : SteelT unit
+    (requires thread_state_inv vs tsm)
+    (ensures fun _ -> thread_state_inv vs (vput_model tsm s v))
+  = let ro = VCache.vcache_get_record vs.st s in
+    match ro with
+    | None ->
+      let _ = fail vs "Slot not found" in
+      change_slprop()
+
+    | Some r ->
+      let x = vcache_update_record vs.st s ({ r with record_value = v }) in
+      change_slprop #(is_vstore _ _ `star` pts_to vs.clock _ _ `star` pts_to vs.failed _ _)// (Mkthread_state_t?.st vs)
+                      //           (hide (Seq.Base.upd (reveal (Mkthread_state_model?.model_store tsm))
+                      //                               (UInt32.v s)
+                      //                               (Some (update_record_value r v)))) `star`
+                      // Steel.Reference.pts_to (Mkthread_state_t?.clock vs)
+                      //                        full_perm
+                      //                        (Mkthread_state_model?.model_clock tsm))
+                    #(thread_state_inv vs (vput_model tsm s v))
+                    ()
+
+val epoch_of_timestamp (t:timestamp) : U32.t
+
+val model_update_hash (tsm:thread_state_model) (r:record) (t:timestamp) (thread_id:thread_id)
+  : tsm':thread_state_model{tsm.model_store == tsm'.model_store}
+val update_hash (#tsm:_) (r:record) (t:timestamp) (thread_id:thread_id) (vs:thread_state_t)
+  : SteelT unit
+    (thread_state_inv vs tsm)
+    (fun _ -> thread_state_inv vs (model_update_hash tsm r t thread_id))
+
+open FStar.Integers
+
+let model_update_clock (tsm:thread_state_model) (ts:timestamp)
+  : thread_state_model
+  = if FStar.UInt.fits (U64.v tsm.model_clock + U64.v ts) 64
+    then { tsm with model_clock = tsm.model_clock + ts } //+1
+    else model_fail tsm
+
+let update_clock (#tsm:_) (ts:timestamp) (vs:thread_state_t)
+  : SteelT unit
+    (thread_state_inv vs tsm)
+    (fun _ -> thread_state_inv vs (model_update_clock tsm ts))
+  = sladmit()
+
+let mk_record k v am = { record_key = k; record_value = v; record_add_method = am;
+                         record_l_child_in_store = Vfalse;
+                         record_r_child_in_store = Vfalse }
+let vaddb_model (tsm:thread_state_model) (s:slot tsm) (r:record) (t:timestamp) (thread_id:thread_id)
+  : thread_state_model
+  = let e = epoch_of_timestamp t in
+    let { record_key = k;
+          record_value = v } = r in
+    (* check value type consistent with key k *)
+    if not (is_value_of k v) then model_fail tsm
+    else if Some? (model_get_record tsm s) then model_fail tsm
+    else (
+      //TODO: need to check that the key does not exist
+      (* updated h_add *)
+      let tsm = model_update_hash tsm r t thread_id in
+      (* updated clock *)
+      let tsm = model_update_clock tsm t in
+      (* add record to store *)
+      model_put_record tsm s (mk_record k v BAdd)
+    )
+
+let vaddb (#tsm:_)
+          (s:slot tsm)
+          (r:record)
+          (t:timestamp)
+          (thread_id:thread_id)
+          (vs:thread_state_t)
+  : SteelT unit
+    (requires thread_state_inv vs tsm)
+    (ensures fun _ -> thread_state_inv vs (vaddb_model tsm s r t thread_id))
+  = (* epoch of timestamp of last evict *)
+    let e = epoch_of_timestamp t in
+    let { record_key = k;
+          record_value = v } = r in
+    (* check value type consistent with key k *)
+    if not (is_value_of k v)
+    then (
+      fail vs "vaddm: value is incompatible with key";
+      change_slprop #(thread_state_inv vs _)
+                    #(thread_state_inv vs _)
+                    ()
+    )
+    else (
+      let ro = VCache.vcache_get_record vs.st s in
+      if Some? ro
+      then (
+        fail vs "vaddm: slot s already exists";
+        change_slprop #(thread_state_inv _ _)
+                      #(thread_state_inv _ _)
+                      ()
+      )
+      else (
+        update_hash r t thread_id vs;
+        update_clock t vs;
+        //this next line is tricky for a couple of reasons
+        // 1. the implicit arg to vcache_update_record is unified with the type of `s` which is indexed
+        //    by the original tsm, not the current one
+        // 2. the refinement type mk_record require `is_value_of k v` does not seem to be provable
+        //    here. despite the check above.
+        VCache.vcache_update_record #((model_update_clock _ _).model_store) vs.st s (mk_record k v BAdd);
+        change_slprop #(is_vstore _ _ `star` pts_to vs.clock _ _ `star` pts_to vs.failed _ _)
+                      #(thread_state_inv vs (vaddb_model tsm s r t thread_id))
+                      ()
+      )
+    )
+
+// let vevictb (s:slot_id) (t:timestamp) (vs:thread_state_t)
+//   : StackExn unit
+//     (requires fun h -> thread_state_inv vs h)
+//     (ensures fun h0 _ h1 -> thread_state_inv vs h1)
+//   = let e = epoch_of_timestamp in
+//     let clk = B.index vs.clock 0ul in
+//     if not (clk `timestamp_lt` t) then raise "vevictb: timestamp does not exceed the clock";
+//     (* check that the vstore contains s *)
+//     let r = vstore_get_record vs.st s in
+//     (* update the evict hash *)
+//     multiset_hash_upd r t vs.id vs.hevict;
+//     (* advance clock to t *)
+//     update_clock t vs.clock;
+//     (* evict record *)
+//     vstore_evict_record vs.st s r.record_key
+
+// let vevictbm (s s':slot_id) (t:timestamp) (vs:thread_state_t)
+//   : StackExn unit
+//     (requires fun h -> thread_state_inv vs h)
+//     (ensures fun h0 _ h1 -> thread_state_inv vs h1)
+//   = let r = vstore_get_record vs.st s in
+//     let r' = vstore_get_record vs.st s' in
+//     match is_descendent r.record_key r'.record_key with
+//     | Some Eq
+//     | None -> raise "vevictbm: Not a proper descendant"
+//     | Some lr ->
+//       assume (V_mval? r'.record_value);
+//       let dh' = desc_hash_dir r'.record_value lr in
+//       match dh' with
+//       | Dh_vnone _ -> raise "vevictbm: parent entry is empty for this child"
+//       | Dh_vsome ({ dhd_key = k2; dhd_h = h2; evicted_to_blum = b2 ;}) ->
+//         if k2 = r.record_key && b2 = Vfalse then
+//            let v'_upd = update_merkle_value r'.record_value lr (Dh_vsome ({ dhd_key = r.record_key; dhd_h = h2; evicted_to_blum = Vtrue; })) in
+//            let r' = { r with record_value = v'_upd } in
+//            vstore_update_record vs.st s' r';
+//            vevictb s t vs
+//         else raise "vevictbm: evicted to blum is already set in parent"
